\documentclass{article}
\usepackage{epsfig}
\usepackage{amsmath}
\usepackage{amsfonts}
\pagestyle{empty}
\begin{document}
\[ \hat{f}(x) = \frac{1}{nh} \sum_{j=1}^n K\Big(\frac{x-x_j}{h}\Big),\]
\pagebreak

$ K $
\pagebreak

$ R $
\pagebreak

$ R^2 $
\pagebreak

$ f: B \subset R \rightarrow R $
\pagebreak

$ \mathbf{q}: B \subset R^n \rightarrow R^m $
\pagebreak

$ \sigma_y^2 $
\pagebreak

$ \sigma_y^2 = \frac{1}{n} \sum_{i=1}^n \left(y_i - \mu \right)^2 $
\pagebreak

$ \mu $
\pagebreak

$ n $
\pagebreak

$ \sigma^2 $
\pagebreak

$ \sigma^2 = \frac{1}{n-1} \sum_{i=1}^n \left(y_i - \mu \right)^2 $
\pagebreak

$ B $
\pagebreak

$ R^n $
\pagebreak

$ R^m $
\pagebreak

$ \pi: B \subset R^n \rightarrow R $
\pagebreak

\[ ||Av|| = ||v|| \]
\pagebreak

\[ min( ||Ax - b||^2) = min(||Ax - b||) = min(||U D V^T x - b||) = min(||D V x - U b||)\]
\pagebreak

\[ y = V^T x \]
\pagebreak

\[ b' = U^T b \]
\pagebreak

\[ Dy = b'\]
\pagebreak

\[ y = inv(D) U^T b \]
\pagebreak

\[ V^T x = y\]
\pagebreak

\[f(x) = y_1 + m (x - x_1), \]
\pagebreak

$ m $
\pagebreak

$(x_1,y_1)$
\pagebreak

\[ f(x)=ax^2+bx+c,\quad a \ne 0.\]
\pagebreak

$ f(x) = y $
\pagebreak

$ P(x) $
\pagebreak

$ \leq n-1 $
\pagebreak

$ (x_1,y_1=f(x_1)), (x_2,y_2=f(x_2)), ..., (x_n,y_n=f(x_n))$
\pagebreak

\[ P(x)=\sum_{j=1}^n \prod_{k=1; k\not=j}^n \frac{x-x_k}{x_j-x_k}.\]
\pagebreak

\[ P(x)=\frac{(x-x_2)(x-x_3)...(x-x_n)}{(x_1-x_2)(x_1-x_3)...(x_1-x_n)}y_1+ \frac{(x-x_1)(x-x_3)...(x-x_n)}{(x_2-x_1)(x_2-x_3)...(x_2-x_n)}y_2+...+ \frac{(x-x_1)(x-x_2)...(x-x_(n-1))}{(x_n-x_1)(x_n-x_2)...(x_n-x_(n-1))}y_n.\]
\pagebreak

$ x_1, x_2, ... x_n $
\pagebreak

$ y_1, y_2, ... y_n $
\pagebreak

$ k+1 $
\pagebreak

$(x_0, y_0),\ldots,(x_j, y_j),\ldots,(x_k, y_k)$
\pagebreak

$ x_j $
\pagebreak

\[ L(x) = \sum_{j=0}^{k} y_j \ell_j(x) \]
\pagebreak

\[ \ell_j(x) = \prod_{0\le m\le k;\, m\neq j} \frac{x-x_m}{x_j-x_m} = \frac{(x-x_0)}{(x_j-x_0)} \cdots \frac{(x-x_{j-1})}{(x_j-x_{j-1})} \frac{(x-x_{j+1})}{(x_j-x_{j+1})} \cdots \frac{(x-x_k)}{(x_j-x_k)},\]
\pagebreak

$ 0\le j\le k $
\pagebreak

$ \ell_j(x) $
\pagebreak

$ j $
\pagebreak

$ x_1 $
\pagebreak

$ f(x) = y_1 + m (x - x_1)$
\pagebreak

$ y_1 $
\pagebreak

$ m$
\pagebreak

$f(x) = y_1 + m (x - x_1)$
\pagebreak

$ x_1i $
\pagebreak

$ f_i(x) = y_{1i} + m_i (x - x_{1i})$
\pagebreak

$ i $
\pagebreak

$ y_{1i} $
\pagebreak

$ m_i $
\pagebreak

$ f(x)=ax^2+bx+c $
\pagebreak

$ a $
\pagebreak

$ b $
\pagebreak

$ c $
\pagebreak

$ f(x)$
\pagebreak

$ g(x)$
\pagebreak

$ W(x)$
\pagebreak

\[\int_{-1}^1 f(x) \, dx = \int_{-1}^1 W(x) g(x) \, dx\]
\pagebreak

$ x_i $
\pagebreak

$ w_i $
\pagebreak

\[ \int_{-1}^1 W(x) g(x) \, dx \approx \sum_{i=1}^n w_i g(x_i) \]
\pagebreak

$ W(x) = 1 $
\pagebreak

$ f(x) $
\pagebreak

\[ \int_{-1}^1 f(x)\,dx \approx \sum_{i=1}^n w_i f(x_i) \]
\pagebreak

$ P_n(x)$
\pagebreak

\[ w_i = \frac{2}{(1-x_i^2)[P'_n(x_i)]^2}=\frac{2(1-x_i^2)}{(n+1)^2[P_{n+1}(x_i)]^2} \]
\pagebreak

$ \pm \frac{1}{3}\sqrt{3} $
\pagebreak

$ 1 $
\pagebreak

$ 0 $
\pagebreak

$ \frac{8}{9} $
\pagebreak

$ \pm \frac{1}{5} \sqrt{15} $
\pagebreak

$ \frac{5}{9} $
\pagebreak

$ \pm \frac{1}{35}\sqrt{525-70\sqrt{30}} $
\pagebreak

$ \frac{1}{36}(18+\sqrt{30})$
\pagebreak

$ \pm \frac{1}{35}\sqrt{525+70\sqrt{30}} $
\pagebreak

$ \frac{1}{36}(18-\sqrt{30})$
\pagebreak

$ \frac{128}{225}$
\pagebreak

$ \pm \frac{1}{21}\sqrt{245-14\sqrt{70}} $
\pagebreak

$ \frac{1}{900}(322+13\sqrt{70})$
\pagebreak

$ \pm \frac{1}{21}\sqrt{245+14\sqrt{70}} $
\pagebreak

$ \frac{1}{900}(322-13\sqrt{70})$
\pagebreak

$(-\infty,\infty)$
\pagebreak

$ W(x)=e^{-x^2}$
\pagebreak

$ H_n(x)$
\pagebreak

$\pm \frac{1}{2}\sqrt{2} $
\pagebreak

$ \frac{1}{2}\sqrt{\pi} $
\pagebreak

$ \frac{2}{3}\sqrt{\pi} $
\pagebreak

$\pm \frac{1}{2}\sqrt{6} $
\pagebreak

$ \frac{1}{6}\sqrt{\pi} $
\pagebreak

$\pm \sqrt{\frac{3-\sqrt{6}}{2}} $
\pagebreak

$ \frac{\sqrt{\pi}}{4(3-\sqrt{6})} $
\pagebreak

$ \frac{\sqrt{\pi}}{4(3+\sqrt{6})} $
\pagebreak

$ W(x)=\frac{1}{\sqrt{1-x^2}}$
\pagebreak

$ T_n(x) $
\pagebreak

$ x_i=\cos[\frac{(2i-1)\pi}{2n}]$
\pagebreak

$ w_i=\frac{\pi}{n}. $
\pagebreak

$ W(x)=\sqrt{1-x^2}$
\pagebreak

$ U_n(x) $
\pagebreak

$ x_i=\cos[\frac{i\pi}{n+1}].$
\pagebreak

$ w_i=\frac{\pi}{n+1}\sin^2[\frac{i\pi}{n+1}]. $
\pagebreak

\[ \int_{\Omega} f(x) \; dx \approx \sum_{i=1}^N f(x_i) w_i \]
\pagebreak

\[ x_j = \sum_{k=0}^{N-1} z_k \exp(-2\pi i j k / N) \]
\pagebreak

$ Ab $
\pagebreak

$ O(N^2)$
\pagebreak

$ N $
\pagebreak

$ A $
\pagebreak

$ f_1 f_2 ... f_n $
\pagebreak

$ O(N \sum f_i) $
\pagebreak

$ O(N \log_2 N)$
\pagebreak

$ O(\c fftSize ^2) $
\pagebreak

$ x = FFT(z) $
\pagebreak

\[ x_j = \sum_{k=0}^{N-1} z_k \exp(-2\pi i j k / N). \]
\pagebreak

$ O(fftSize^2) $
\pagebreak

$ x = IFFT(z)$
\pagebreak

\[ z_j = {1 \over N} \sum_{k=0}^{N-1} x_k \exp(2\pi i j k / N).\]
\pagebreak

$ 1/N $
\pagebreak

$ <f> = 1/|\Omega| \int_{\Omega} f(x) \; dx $
\pagebreak

\[ \int_{\Omega} f(x) \; dx = |\Omega| <f> \approx |\Omega| \frac{1}{N} \sum_{i=1}^N f(x_i) \]
\pagebreak

$N$
\pagebreak

$|\Omega|/N $
\pagebreak

$ \sum_{i=1}^N f(x_i) w_i $
\pagebreak

$ lnValue = \sum[ (alpha_i-1)*log(domainVector_i) + (beta_i-1)*log(1-domainVector_i)] + m_logOfNormalizationFactor $
\pagebreak

\[ y=f(x|a,b)= \frac{1}{B(a,b)} x^{a-1}(1-x)^{b-1}, \]
\pagebreak

\[ B(a,b)=\frac{\Gamma(a)\Gamma(b)}{\Gamma(a+b)}=\frac{(a-1)!(b-1)!}{(a+b-1)!}.\]
\pagebreak

\[ cov = a \exp{(-d^2/\sigma^2)}\]
\pagebreak

$ d=d(x,y) $
\pagebreak

$ cov= a exp (-d^2/sigma)$
\pagebreak

$ d= \sqrt{(domainVector1 - domainVector1)^2} $
\pagebreak

\[ f(x) = C x^{a-1} \exp \left( x / b \right), \]
\pagebreak

$\theta$
\pagebreak

$ lnValue = \sum[ (a_i-1)*log(domainVector_i) -domainVector_i/b_i + m_logOfNormalizationFactor $
\pagebreak

\[ y = f(x|a,b) = \frac{1}{b^{a}\Gamma(a)} x^{a-1} e^{\frac{x}{b}}, \]
\pagebreak

$ \Gamma(.) $
\pagebreak

\[ B(a,b) = \frac{\Gamma(a)\Gamma(b)}{\Gamma(a+b)} = \frac{(a-1)!(b-1)!}{(a+b-1)!}. \]
\pagebreak

$ (0, \infty)$
\pagebreak

\[ lnValue =- \sum_i \frac{1}{\sqrt{|covMatrix|} \sqrt{2 \pi}} exp(-\frac{(domainVector_i - lawExpVector_i)* covMatrix^{-1}* (domainVector_i - lawExpVector_i) }{2}, \]
\pagebreak

$ covMatrix $
\pagebreak

\[ f(x| \mu,\sigma) = \frac{1}{\sigma\sqrt{2\pi}} e^{ -\frac{(x-\mu)^2}{2\sigma^2} }. \]
\pagebreak

$ \sigma $
\pagebreak

\[ y=f(x| a,b)= \frac{b^a}{\Gamma(a)} x^{-a - 1}\exp\left(-\frac{b}{x}\right)\]
\pagebreak

\[ p(x) = \frac{1}{2 \sigma^2 \pi} \exp \left( - \frac12 (\mbox{logit} x - \mu)^2 \right) \mbox{logit}'(x), \quad x \in [a, b], \]
\pagebreak

\[ \mbox{logit}(x) = \log \left( \frac{x - a}{b - x} \right), \quad x \in [a, b]. \]
\pagebreak

\[ lnValue =- \sum_i \frac{1}{\sqrt{|covMatrix|} \sqrt{2 \pi}} exp(-\frac{(domainVector_i - lawExpVector_i) * covMatrix^{-1} * (domainVector_i - lawExpVector_i) }{2} + \log \mbox{logit}'(domainVector_i), \]
\pagebreak

$ f(X) $
\pagebreak

$ X $
\pagebreak

\[ f(x) = \frac{b \exp(x) + a}{1 + \exp(x)}. \]
\pagebreak

\[ lnValue =- \sum_i \frac{1}{domainVector_i * \sqrt{2 \pi * lawVarVector_i}} exp(-\frac{(\ln( domainVector_i) - lawExpVector_i)^2}{2 lawVarVector_i}) \]
\pagebreak

$ domainVector_i > 0 $
\pagebreak

\[ f(x|\mu,\sigma) = \frac{1}{x \sigma \sqrt{2 \pi}}\, e^{-\frac{(\ln x - \mu)^2}{2\sigma^2}}, x>0 \]
\pagebreak

$ 1/scales^2 $
\pagebreak

$ ln( \pi(D|M) ) = E[ln( \pi(D|\theta,M) )] - E[ln( \pi(\theta|D,M) / \pi(\theta|M) )] $
\pagebreak

\[ \pi (\theta|D, M_j) = \frac{f(D|\theta, M_j) \cdot \pi (\theta | M_j)}{\pi(D, M_j)} \]
\pagebreak

$ \pi (\theta|D, M_j) $
\pagebreak

$ \pi (\theta | M_j) $
\pagebreak

$ f(D|\theta, M_j)$
\pagebreak

$ \pi(D, M_j) $
\pagebreak

$ \theta $
\pagebreak

$ D $
\pagebreak

$ M_j $
\pagebreak

\[ EIG = log \left(\frac{ \pi (\theta|D, M_j)}{\pi (\theta | M_j) } \right) = log \left(\frac{f(D|\theta, M_j) }{\pi(D, M_j)} \right) = log \left(\frac{f(D|\theta, M_j) }{\pi(D, M_j)} \right) = log \left(f(D|\theta, M_j)\right) - log\left(f(D|\theta, M_j) \right) \]
\pagebreak

$ f: B \subset R \rightarrow C \subset R $
\pagebreak

$ C = [0,1]$
\pagebreak

$ Y $
\pagebreak

$ cov (X,Y) = <(X-\mu_X)(Y-\mu_Y)> = < X Y > - \mu_X \mu_Y $
\pagebreak

$ \mu_X $
\pagebreak

$ \mu_Y $
\pagebreak

\[ cov (X,Y) = \sum_{i=1}^{N} \frac{(x_i - \bar{x})(y_i - \bar{y})}{N}\]
\pagebreak

$ q() $
\pagebreak

$ x $
\pagebreak

$ q(x) $
\pagebreak

$ \pi()$
\pagebreak

$ \pi(x) $
\pagebreak

$ \ln[\pi(x)] $
\pagebreak

$ x \in R^n $
\pagebreak

$ A \in B $
\pagebreak

$ P(x,R^n)=1 $
\pagebreak

$ P(x, {x}) $
\pagebreak

$ X_1, X_2, ..., X_n $
\pagebreak

$ X_i $
\pagebreak

$ n$
\pagebreak

$ f: \mathbb{R}^n \rightarrow \mathbb{R} $
\pagebreak

$ \sum_{ijkl...} f_{ijkl...} N_{ijkl...} $
\pagebreak

$ ijkl... $
\pagebreak

$ N_{ijkl...} (\xi, \eta, \zeta,...) = N_i(\eta) N_j(\eta) N_k(\zeta) ... $
\pagebreak

\end{document}
